code/kyber2/impl/Spec.Kyber2.NTT.fst
@@ -20,16 +20,8 @@ open Lib.Poly.NTT2
 module Seq = Lib.Sequence
 module Loops = Lib.LoopCombinators
 
-
-type reversed (#m:nat) (a:poly m) = bool
-type normal (#m:nat) (a:poly m) = bool
-
 type zq = field params_q
-unfold inline_for_extraction 
-type nttpoly = p:(poly params_q){reversed p}
-
-unfold inline_for_extraction
-type poly  =  p:(poly params_q){normal p}
+let ring_zq = Lib.Arithmetic.Ring.ring_mod #params_q
 
 #reset-options "--z3rlimit 100 --max_fuel 1 --max_ifuel 1 --using_facts_from '* -FStar.Seq'"
 
@@ -46,17 +38,17 @@ let lemma_is_prime_params_q () =
 
 val ntt:
   p:poly
-  -> Tot (p':nttpoly)
+  -> Tot (p':poly)
 
 let ntt p =
-  let p': nttpoly = lib_ntt params_zeta p in p'
+  let p': poly = lib_ntt #Spec.Kyber2.Group.t #Spec.Kyber2.Ring.ring_t #params_n 7 (i16 params_zeta) p in p'
 
 val nttinv:
-  p:nttpoly
+  p:poly
   -> Tot (p':poly)
 
 let nttinv p =
-  let p':poly = lib_nttinv params_halfninv params_zetainv p in p'
+  let p':poly = lib_nttinv #Spec.Kyber2.Group.t #Spec.Kyber2.Ring.ring_t #params_n 7 (i16 params_halfninv) (i16 params_zetainv) p in p'
 
 
 
@@ -92,7 +84,7 @@ let order_zeta unit =
     assert(acc *% (params_zeta ^% (p+1)) = 1);
     let customprop (d:nat{d<p+1}) : Type0 = (d>0 \/ counter > 0) ==> acc *% (params_zeta ^% d) <> 1 in
     let customlemma (d:nat{d<p+1}) : Lemma (customprop d) =
-      if d=0 then 
+      if d=0 then
 	if acc = 1 then (assert(counter = 0); ())
 	  else (modular_exp_lemma_zero #params_q params_zeta; modular_mul_one_lemma #params_q acc; assert (acc *% (params_zeta ^% d) = acc); ())
       else
@@ -119,30 +111,112 @@ let order_zeta unit =
   FStar.Classical.forall_intro lemma_p;
   p
 
-val lemma_multiplicative_order_zeta: unit -> Lemma (forall (nn:field (params_n)). params_zeta ^% nn = 1 ==> nn = 0)
+val lemma_multiplicative_order_params_zeta: unit -> Lemma (forall (nn:nat{nn<params_n}). params_zeta ^% nn = 1 ==> nn = 0)
 
-let lemma_multiplicative_order_zeta () =
+let lemma_multiplicative_order_params_zeta () =
   assert_norm(order_zeta () = params_n); ()
 
+let exp_t = Lib.Arithmetic.Ring.exp #Group.t #Ring.ring_t
 
+let rec exp_correspondancy (a:Group.t) (n:nat) : Lemma (ensures Group.v (exp_t a n) == (Group.v a) ^% n) (decreases n) =
+  if n = 0 then Lib.Arithmetic.Ring.lemma_exp_zero #Group.t #Ring.ring_t a
+  else (Lib.Arithmetic.Ring.lemma_exp_succ1 #Group.t #Ring.ring_t a (n-1); Group.mul_lemma_t a (exp_t a (n-1)); exp_correspondancy a (n-1))
 
-#reset-options "--z3rlimit 200 --max_fuel 0 --max_ifuel 0 --using_facts_from '* -FStar.Seq'"
-val ntt_inversion_lemma: 
+let repeat_plus_t = Lib.Arithmetic.Ring.repeat_plus #Group.t #Ring.ring_t
+let repeat_plus_zq = Lib.Arithmetic.Ring.repeat_plus #(field params_q) #(Lib.Arithmetic.Ring.ring_mod #params_q)
+
+let rec repeat_plus_correspondancy (a:Group.t) (n:nat) : Lemma (ensures Group.v (repeat_plus_t a n) == repeat_plus_zq (Group.v a) n) (decreases n) =
+  if n = 0 then (Lib.Arithmetic.Group.lemma_repeat_op_zero #Group.t #(Group.monoid_plus_t) a; Lib.Arithmetic.Group.lemma_repeat_op_zero #(field params_q) #(Lib.Arithmetic.Group.monoid_plus_mod #params_q) (Group.v a))
+  else (Lib.Arithmetic.Group.lemma_repeat_op_succ1 #Group.t #Group.monoid_plus_t a (n-1); Lib.Arithmetic.Group.lemma_repeat_op_succ1 #(field params_q) #(Lib.Arithmetic.Group.monoid_plus_mod #params_q) (Group.v a) (n-1); Group.plus_lemma_t a (repeat_plus_t a (n-1)); repeat_plus_correspondancy a (n-1))
+
+val lemma_multiplicative_order_zeta: unit -> Lemma (forall (nn:nat{nn<params_n}). exp_t (Group.mk_t params_zeta) nn == Group.one_t ==> nn = 0)
+
+let lemma_multiplicative_order_zeta () =
+  let customprop (nn:nat{nn<params_n}) : Type0 = (exp_t (Group.mk_t params_zeta) nn == Group.one_t ==> nn = 0) in
+  let customlemma (nn:nat{nn<params_n}) : Lemma (customprop nn) =
+    exp_correspondancy (Group.mk_t params_zeta) nn;
+    lemma_multiplicative_order_params_zeta ()
+  in FStar.Classical.forall_intro customlemma
+
+#reset-options "--z3rlimit 500 --max_fuel 1 --max_ifuel 1 --using_facts_from '* -FStar.Seq'"
+
+val lemma_is_invertible_implication : (a:Group.t) -> Lemma (requires ~(Lib.Arithmetic.Ring.is_invertible #Group.t #Ring.ring_t a)) (ensures ~(is_invertible #params_q (Group.v a)))
+
+let lemma_is_invertible_implication a =
+  let customprop (y:field params_q) : Type0 = (~((Group.v a) *% y = 1)) in
+  let customlemma (y:field params_q) : Lemma (customprop y) =
+    if((Group.v a) *% y = 1) then (Group.mul_lemma_t a (Group.mk_t y); Ring.lemma_mul_swap_t a (Group.mk_t y); assert(Group.mul_t a (Group.mk_t y) == Group.one_t /\ Group.mul_t (Group.mk_t y) a == Group.one_t); FStar.Classical.exists_intro (fun y -> Group.mul_t a y == Group.one_t) (Group.mk_t y)) else () in
+  FStar.Classical.forall_intro customlemma
+
+  #reset-options "--z3rlimit 200 --max_fuel 0 --max_ifuel 0 --using_facts_from '* -FStar.Seq'"
+val ntt_inversion_lemma1:
  p:poly
  -> Lemma(nttinv (ntt p) == p)
 
-let ntt_inversion_lemma p =
+let ntt_inversion_lemma1 p =
   lemma_is_prime_params_q ();
   assert_norm(order_zeta () = params_n);
-  lemma_multiplicative_order_zeta ();
-  let customprop' (nn:field (params_n)) : Type0 = (~(is_invertible((params_zeta ^% nn) -%1)) ==> nn = 0) in
+  lemma_multiplicative_order_params_zeta ();
+  let customprop' (nn:field (params_n)) : Type0 = (~(Lib.Arithmetic.Ring.is_invertible #Group.t #Ring.ring_t (Lib.Arithmetic.Ring.minus #Group.t #Ring.ring_t (exp_t (Group.mk_t params_zeta) nn) Group.one_t)) ==> nn = 0) in
   let customlemma' (nn:field (params_n)) : Lemma (customprop' nn) =
+     exp_correspondancy (Group.mk_t params_zeta) nn;
+     Ring.minus_lemma_t (exp_t (Group.mk_t params_zeta) nn) Group.one_t;
+     assert(Group.v (Lib.Arithmetic.Ring.minus #Group.t #Ring.ring_t (exp_t (Group.mk_t params_zeta) nn) Group.one_t) == (params_zeta ^% nn) -% 1);
+     FStar.Classical.move_requires lemma_is_invertible_implication (Lib.Arithmetic.Ring.minus #Group.t #Ring.ring_t (exp_t (Group.mk_t params_zeta) nn) Group.one_t);
+     assert(~(Lib.Arithmetic.Ring.is_invertible #Group.t #Ring.ring_t (Lib.Arithmetic.Ring.minus #Group.t #Ring.ring_t (exp_t (Group.mk_t params_zeta) nn) Group.one_t)) ==> ~(is_invertible #params_q ((params_zeta ^% nn) -% 1)));
      lemma_q_prime_zq_field params_q
      in
   FStar.Classical.forall_intro customlemma';
-  lib_ntt_inversion_lemma_with_explicit_inverses params_halfninv params_zeta params_zetainv p
+  assert_norm (repeat_plus_zq 1 (params_n/2) == params_n/2);
+  repeat_plus_correspondancy Group.one_t (params_n/2);
+  shift_right_lemma (Group.mk_t params_n) (size 1);
+  assert(params_halfninv *% repeat_plus_zq 1 (params_n/2) = 1);
+  Group.mul_lemma_t (Group.mk_t params_halfninv) (repeat_plus_t Group.one_t (params_n/2));
+  assert(Group.mul_t (Group.mk_t params_halfninv) (repeat_plus_t Group.one_t (params_n/2)) == Group.one_t);
+  lemma_multiplicative_order_zeta ();
+  Group.mul_lemma_t (Group.mk_t params_zeta) (Group.mk_t params_zetainv);
+  Ring.lemma_mul_swap_t (Group.mk_t params_zeta) (Group.mk_t params_zetainv);
+  assert(op_Star_Percent #params_q params_zeta params_zetainv = 1);
 
+  assert(Lib.Arithmetic.Ring.mul #Group.t #Ring.ring_t (Group.mk_t params_halfninv) (Lib.Arithmetic.Ring.repeat_plus #Group.t #Ring.ring_t (Lib.Arithmetic.Ring.one #Group.t #Ring.ring_t) (params_n/2)) == Lib.Arithmetic.Ring.one #Group.t #Ring.ring_t);
+  exp_correspondancy (Group.mk_t params_zeta) params_n;
+  assert(Lib.Arithmetic.Ring.exp #Group.t #Ring.ring_t (Group.mk_t params_zeta) params_n == Lib.Arithmetic.Ring.one #Group.t #Ring.ring_t);
+  assert_norm(Lib.Poly.NTT.lib_poly Group.t params_n == poly);
+  let coerce #a #b (x:a) : Pure b (requires a == b) (ensures fun _ -> True) = x in
+  lib_ntt_inversion_lemma1 #Group.t #Ring.ring_t #params_n 7 (Group.mk_t params_halfninv) (Group.mk_t params_zeta) (Group.mk_t params_zetainv) (coerce p)
 
-//val forall_elim: #a:Type0 -> #p: (a -> Type0) -> (squash (forall(y:a). p y)) -> (y:a -> Lemma (p y))
-//let forall_elim #a #p s = fun y -> (give_witness_from_squash s; assert(p y))
+val ntt_inversion_lemma2:
+ p:poly
+ -> Lemma(ntt (nttinv p) == p)
 
+let ntt_inversion_lemma2 p =
+  lemma_is_prime_params_q ();
+  assert_norm(order_zeta () = params_n);
+  lemma_multiplicative_order_params_zeta ();
+  let customprop' (nn:field (params_n)) : Type0 = (~(Lib.Arithmetic.Ring.is_invertible #Group.t #Ring.ring_t (Lib.Arithmetic.Ring.minus #Group.t #Ring.ring_t (exp_t (Group.mk_t params_zeta) nn) Group.one_t)) ==> nn = 0) in
+  let customlemma' (nn:field (params_n)) : Lemma (customprop' nn) =
+     exp_correspondancy (Group.mk_t params_zeta) nn;
+     Ring.minus_lemma_t (exp_t (Group.mk_t params_zeta) nn) Group.one_t;
+     assert(Group.v (Lib.Arithmetic.Ring.minus #Group.t #Ring.ring_t (exp_t (Group.mk_t params_zeta) nn) Group.one_t) == (params_zeta ^% nn) -% 1);
+     FStar.Classical.move_requires lemma_is_invertible_implication (Lib.Arithmetic.Ring.minus #Group.t #Ring.ring_t (exp_t (Group.mk_t params_zeta) nn) Group.one_t);
+     assert(~(Lib.Arithmetic.Ring.is_invertible #Group.t #Ring.ring_t (Lib.Arithmetic.Ring.minus #Group.t #Ring.ring_t (exp_t (Group.mk_t params_zeta) nn) Group.one_t)) ==> ~(is_invertible #params_q ((params_zeta ^% nn) -% 1)));
+     lemma_q_prime_zq_field params_q
+     in
+  FStar.Classical.forall_intro customlemma';
+  assert_norm (repeat_plus_zq 1 (params_n/2) == params_n/2);
+  repeat_plus_correspondancy Group.one_t (params_n/2);
+  shift_right_lemma (Group.mk_t params_n) (size 1);
+  assert(params_halfninv *% repeat_plus_zq 1 (params_n/2) = 1);
+  Group.mul_lemma_t (Group.mk_t params_halfninv) (repeat_plus_t Group.one_t (params_n/2));
+  assert(Group.mul_t (Group.mk_t params_halfninv) (repeat_plus_t Group.one_t (params_n/2)) == Group.one_t);
+  lemma_multiplicative_order_zeta ();
+  Group.mul_lemma_t (Group.mk_t params_zeta) (Group.mk_t params_zetainv);
+  Ring.lemma_mul_swap_t (Group.mk_t params_zeta) (Group.mk_t params_zetainv);
+  assert(op_Star_Percent #params_q params_zeta params_zetainv = 1);
+
+  assert(Lib.Arithmetic.Ring.mul #Group.t #Ring.ring_t (Group.mk_t params_halfninv) (Lib.Arithmetic.Ring.repeat_plus #Group.t #Ring.ring_t (Lib.Arithmetic.Ring.one #Group.t #Ring.ring_t) (params_n/2)) == Lib.Arithmetic.Ring.one #Group.t #Ring.ring_t);
+  exp_correspondancy (Group.mk_t params_zeta) params_n;
+  assert(Lib.Arithmetic.Ring.exp #Group.t #Ring.ring_t (Group.mk_t params_zeta) params_n == Lib.Arithmetic.Ring.one #Group.t #Ring.ring_t);
+  assert_norm(Lib.Poly.NTT.lib_poly Group.t params_n == poly);
+  let coerce #a #b (x:a) : Pure b (requires a == b) (ensures fun _ -> True) = x in
+  lib_ntt_inversion_lemma2 #Group.t #Ring.ring_t #params_n 7 (Group.mk_t params_halfninv) (Group.mk_t params_zeta) (Group.mk_t params_zetainv) (coerce p)
