code/kyber2/impl/Impl.Kyber2.NTT.fst
@@ -1,0 +1,32 @@
+module Impl.Kyber2.NTT
+
+open FStar.HyperStack
+open FStar.HyperStack.ST
+
+open Lib.IntTypes
+open Impl.Kyber2.Group
+open Impl.Kyber2.Ring
+open Lib.Buffer
+
+module ST = FStar.HyperStack.ST
+module Buf = Lib.Buffer
+module Seq = Lib.Sequence
+
+open Spec.Kyber2.Params
+
+noextract inline_for_extraction let zeta:t = i16 params_zeta
+
+noextract inline_for_extraction let n2:(x:size_t{v x = params_n/2}) =
+  size params_n >>. size 1
+(*
+let ntt_sequence1 (input:lbuffer t n2) (output:lbuffer t n2) (k:size_t{v k < params_n/2}) : Stack unit
+  (requires fun h -> live h input /\ live h output /\ Buf.disjoint input output)
+  (ensures fun h0 _ h1 -> modifies1 output h0 h1 /\ h1.[|output|] == Lib.Poly.NTT.lib_ntt_sequence #t #Spec.Kyber2.Ring.ring_t (Lib.Arithmetic.Ring.exp #t #Spec.Kyber2.Ring.ring_t zeta 2) zeta h0.[|input|] (v k)) = 
+  let h = ST.get () in
+  mapiT output (fun i g -> mul_t (exp_t 
+(*
+let ntt1 (input:lbuffer t (size params_n >>. size 2)) (output:lbuffer t (size params_n >>. size 2)) : Stack unit
+  (requires fun h -> live h input /\ live h output /\ Buf.disjoint input output)
+  (ensures fun h0 _ h1 -> modifies1 output h0 h1 /\ h1.[|output|] == Lib.Poly.NTT.lib_ntt #t #Spec.Kyber2.Ring.ring_t (Lib.Arithmetic.Ring.exp #t #Spec.Kyber2.Ring.ring_t (i16 params_zeta) 2) (i16 params_zeta) h0.[|input|]) =
+  let h0 = ST.get () in
+  Buf.mapiT (size params_n >>. size 2) output (fun j g -> 
