code/kyber2/impl/Spec.Kyber2.NumericTypes.fst
@@ -1,0 +1,91 @@
+module Spec.Kyber2.NumericTypes
+
+open FStar.Mul
+
+open Spec.Kyber2.Params
+open Spec.Powtwo.Lemmas
+open Lib.NumericTypes
+
+open Lib.Sequence
+open Lib.IntTypes
+open Lib.NumericTypes
+
+module Seq = Lib.Sequence
+
+type num_t = Base Group.t
+type poly_t = vector_t #num_t params_n
+type vec_t = vector_t #poly_t params_k
+type matrix_t = matrix_t #poly_t params_k params_k
+
+type num = Group.t
+type poly = vector_i #num_t params_n
+type vec = vector_i #poly_t params_k
+type matrix = matrix_i #poly_t params_k params_k
+
+#reset-options "--z3rlimit 200 --max_fuel 2 --max_ifuel 2 --using_facts_from '* -FStar.Seq'"
+let ring_num = Ring.ring_t
+let ring_poly = Lib.Poly.NTT2.lib_ntt_ring #num #ring_num #params_n 7 (Group.mk_t params_zeta)
+
+let new_poly () : poly = create params_n (Group.zero_t)
+let new_vec () : vec = create params_k (new_poly ())
+let new_matrix () : matrix = create params_k (new_vec ())
+
+let index_vec (v:vec) i : poly = Seq.index #_ #params_k v i
+
+let get_line (m:matrix) i : vec = Seq.index #_ #params_k m i
+
+let get_element (m:matrix) i j : poly = index_vec (get_line m i) j
+
+let get_column (m:matrix) j : vec = Seq.createi params_k (fun i -> get_element m i j)
+
+let upd_vec (v:vec) i (x:poly) : vec = upd #_ #params_k v i x
+
+let upd_line (m:matrix) i (v:vec) : matrix = upd #_ #params_k m i v
+
+let upd_matrix (m:matrix) (i:size_nat{i<params_k}) (j:size_nat{j<params_k}) (x:poly) : matrix = upd_line m i (upd_vec (get_line m i) j x)
+
+let eq_vec (v1:vec) (v2:vec) : Lemma (requires forall i. {:pattern (index_vec v1 i); (index_vec v2 i)} index_vec v1 i == index_vec v2 i) (ensures v1 == v2) =
+  let customprop (i:size_nat{i<params_k}) : Type0 = (Seq.index #_ #params_k v1 i == Seq.index #_ #params_k v2 i) in
+  let customlemma (i:size_nat{i<params_k}) : Lemma (customprop i) = assert(index_vec v1 i == index_vec v2 i)
+  in FStar.Classical.forall_intro customlemma; Seq.eq_intro #_ #params_k v1 v2
+
+let eq_matrix_line (m1:matrix) (m2:matrix) : Lemma (requires forall i. {:pattern (get_line m1 i); (get_line m2 i)} get_line m1 i == get_line m2 i) (ensures m1 == m2) =
+  let customprop (i:size_nat{i<params_k}) : Type0 = (Seq.index #_ #params_k m1 i == Seq.index #_ #params_k m2 i) in
+  let customlemma (i:size_nat{i<params_k}) : Lemma (customprop i) = assert(get_line m1 i == get_line m2 i)
+  in FStar.Classical.forall_intro customlemma; Seq.eq_intro #_ #params_k m1 m2
+
+let eq_matrix_element (m1:matrix) (m2:matrix) : Lemma (requires forall i j. {:pattern (get_element m1 i j); (get_element m2 i j)} get_element m1 i j == get_element m2 i j) (ensures m1 == m2) =
+  let customprop (i:size_nat{i<params_k}) : Type0 = (Seq.index #_ #params_k m1 i == Seq.index #_ #params_k m2 i) in
+  let customlemma (i:size_nat{i<params_k}) : Lemma (customprop i) =
+    let v1:vec = Seq.index #_ #params_k m1 i in
+    let v2:vec = Seq.index #_ #params_k m2 i in
+    let customprop' (j:size_nat{j<params_k}) : Type0 = (Seq.index #_ #params_k v1 j == Seq.index #_ #params_k v2 j) in
+    let customlemma' (j:size_nat{j<params_k}) : Lemma (customprop' j) =
+      assert(get_element m1 i j == get_element m2 i j)
+    in FStar.Classical.forall_intro customlemma';
+    Seq.eq_intro #_ #params_k v1 v2
+  in FStar.Classical.forall_intro customlemma; Seq.eq_intro #_ #params_k m1 m2
+
+let eq_matrix_column (m1:matrix) (m2:matrix) : Lemma (requires forall j. {:pattern (get_column m1 j); (get_column m2 j)} get_column m1 j == get_column m2 j) (ensures m1 == m2) =
+  let b (i:size_nat{i<params_k}) : Type0 = (j:size_nat{j<params_k}) in
+  let customprop (i:size_nat{i<params_k}) (j: b i) : Type0 = (get_element m1 i j == get_element m2 i j) in
+  let customlemma (i:size_nat{i<params_k}) (j: b i) : Lemma (customprop i j) =
+    assert(Seq.index #_ #params_k (get_column m1 j) i == Seq.index #_ #params_k (get_column m2 j) i)
+  in FStar.Classical.forall_intro_2 customlemma; eq_matrix_element m1 m2
+
+inline_for_extraction noextract
+let rec gen_matrix_ (m:matrix) (f: (i:nat{i<params_k}) -> (j:nat{j<params_k}) -> Tot (option poly)) (i:size_nat{i<=params_k}) (j:size_nat{j<=params_k}) : Tot (option matrix) (decreases ((params_k+1)*(params_k+1) -(params_k+1)*i-j)) =
+  if (i=params_k) then Some m
+  else if (j=params_k) then gen_matrix_ m f (i+1) 0
+  else
+  match f i j with
+  |None -> None
+  |Some p -> gen_matrix_ (upd_matrix m i j p) f i (j+1)
+
+val gen_matrix: (f: (i:nat{i<params_k}) -> (j:nat{j<params_k}) -> Tot (option poly)) -> Tot (option matrix)
+
+let gen_matrix f = gen_matrix_ (new_matrix ()) f 0 0
+
+let dot_product (x:vec) (y:vec) = Lib.NumericTypes.dot_product x y
+
+let matrix_vector_product (m:matrix) (v:vec) = createi params_k (fun i -> dot_product (get_line m i) v)
